projects/lib/gmp_goal.v
@@ -15,10 +15,10 @@ Local Open Scope Z_scope.
 Local Open Scope sets.
 Local Open Scope string.
 Local Open Scope list.
+Require Import Coq.ZArith.ZArith.
+Local Open Scope Z_scope.
 Import naive_C_Rules.
 Local Open Scope sac.
-
-Definition Zmax := Z.max.
 
 (*----- Function gmp_abs -----*)
 
@@ -61,7 +61,7 @@ forall (b_pre: Z) (a_pre: Z) ,
   [| (a_pre <= b_pre) |]
   &&  emp
 |--
-  [| (b_pre = (Zmax (a_pre) (b_pre))) |]
+  [| (b_pre = (Z.max (a_pre) (b_pre))) |]
   &&  emp
 .
 
@@ -70,7 +70,7 @@ forall (b_pre: Z) (a_pre: Z) ,
   [| (a_pre > b_pre) |]
   &&  emp
 |--
-  [| (a_pre = (Zmax (a_pre) (b_pre))) |]
+  [| (a_pre = (Z.max (a_pre) (b_pre))) |]
   &&  emp
 .
 
@@ -1753,6 +1753,552 @@ forall (xp_pre: Z) (val: Z) (cap: Z) (n: Z) ,
   **  (store_undef_uint_array_rec xp_pre n cap )
 .
 
+(*----- Function mpn_add_1 -----*)
+
+Definition mpn_add_1_safety_wit_1 := 
+forall (b_pre: Z) (n_pre: Z) (ap_pre: Z) (rp_pre: Z) (cap2: Z) (cap1: Z) (l2: (@list Z)) (val: Z) (l: (@list Z)) ,
+  [| (n_pre <= cap1) |] 
+  &&  [| ((Zlength (l)) = n_pre) |] 
+  &&  [| (cap1 <= 100000000) |] 
+  &&  [| (list_store_Z_compact l val ) |] 
+  &&  [| ((Zlength (l2)) = cap2) |] 
+  &&  [| (cap2 >= n_pre) |] 
+  &&  [| (cap1 <= 100000000) |] 
+  &&  [| (cap2 <= 100000000) |] 
+  &&  [| (n_pre > 0) |] 
+  &&  [| (n_pre <= cap1) |]
+  &&  ((( &( "i" ) )) # Int  |->_)
+  **  (store_uint_array ap_pre n_pre l )
+  **  (store_undef_uint_array_rec ap_pre n_pre cap1 )
+  **  ((( &( "b" ) )) # UInt  |-> b_pre)
+  **  ((( &( "n" ) )) # Int  |-> n_pre)
+  **  ((( &( "ap" ) )) # Ptr  |-> ap_pre)
+  **  ((( &( "rp" ) )) # Ptr  |-> rp_pre)
+  **  (store_uint_array rp_pre cap2 l2 )
+|--
+  [| (0 <= INT_MAX) |] 
+  &&  [| ((INT_MIN) <= 0) |]
+.
+
+Definition mpn_add_1_safety_wit_2 := 
+forall (b_pre: Z) (n_pre: Z) (ap_pre: Z) (rp_pre: Z) (cap2: Z) (cap1: Z) (l2: (@list Z)) (val: Z) (l: (@list Z)) (l'': (@list Z)) (l': (@list Z)) (val2: Z) (val1: Z) (l_2: (@list Z)) (i: Z) ,
+  [| ((unsigned_last_nbits (((Znth i l_2 0) + b_pre )) (32)) >= b_pre) |] 
+  &&  [| (i < n_pre) |] 
+  &&  [| (0 <= i) |] 
+  &&  [| (i <= n_pre) |] 
+  &&  [| (list_store_Z_compact l_2 val ) |] 
+  &&  [| (n_pre <= cap1) |] 
+  &&  [| (list_store_Z (sublist (0) (i) (l_2)) val1 ) |] 
+  &&  [| (list_store_Z l' val2 ) |] 
+  &&  [| ((val2 + (b_pre * (Z.lxor UINT_MOD i) ) ) = (val1 + b_pre )) |] 
+  &&  [| ((Zlength (l2)) = cap2) |] 
+  &&  [| (n_pre <= cap1) |] 
+  &&  [| ((Zlength (l)) = n_pre) |] 
+  &&  [| (cap1 <= 100000000) |] 
+  &&  [| (list_store_Z_compact l val ) |] 
+  &&  [| ((Zlength (l2)) = cap2) |] 
+  &&  [| (cap2 >= n_pre) |] 
+  &&  [| (cap1 <= 100000000) |] 
+  &&  [| (cap2 <= 100000000) |] 
+  &&  [| (n_pre > 0) |] 
+  &&  [| (n_pre <= cap1) |]
+  &&  (store_uint_array_rec rp_pre i cap2 (replace_Znth ((i - i )) ((unsigned_last_nbits (((Znth i l_2 0) + b_pre )) (32))) (l'')) )
+  **  (store_uint_array ap_pre n_pre l_2 )
+  **  ((( &( "r" ) )) # UInt  |-> (unsigned_last_nbits (((Znth i l_2 0) + b_pre )) (32)))
+  **  ((( &( "i" ) )) # Int  |-> i)
+  **  (store_undef_uint_array_rec ap_pre n_pre cap1 )
+  **  (store_uint_array rp_pre i l' )
+  **  ((( &( "b" ) )) # UInt  |-> 0)
+  **  ((( &( "n" ) )) # Int  |-> n_pre)
+  **  ((( &( "ap" ) )) # Ptr  |-> ap_pre)
+  **  ((( &( "rp" ) )) # Ptr  |-> rp_pre)
+|--
+  [| ((i + 1 ) <= INT_MAX) |] 
+  &&  [| ((INT_MIN) <= (i + 1 )) |]
+.
+
+Definition mpn_add_1_safety_wit_3 := 
+forall (b_pre: Z) (n_pre: Z) (ap_pre: Z) (rp_pre: Z) (cap2: Z) (cap1: Z) (l2: (@list Z)) (val: Z) (l: (@list Z)) (l'': (@list Z)) (l': (@list Z)) (val2: Z) (val1: Z) (l_2: (@list Z)) (i: Z) ,
+  [| ((unsigned_last_nbits (((Znth i l_2 0) + b_pre )) (32)) < b_pre) |] 
+  &&  [| (i < n_pre) |] 
+  &&  [| (0 <= i) |] 
+  &&  [| (i <= n_pre) |] 
+  &&  [| (list_store_Z_compact l_2 val ) |] 
+  &&  [| (n_pre <= cap1) |] 
+  &&  [| (list_store_Z (sublist (0) (i) (l_2)) val1 ) |] 
+  &&  [| (list_store_Z l' val2 ) |] 
+  &&  [| ((val2 + (b_pre * (Z.lxor UINT_MOD i) ) ) = (val1 + b_pre )) |] 
+  &&  [| ((Zlength (l2)) = cap2) |] 
+  &&  [| (n_pre <= cap1) |] 
+  &&  [| ((Zlength (l)) = n_pre) |] 
+  &&  [| (cap1 <= 100000000) |] 
+  &&  [| (list_store_Z_compact l val ) |] 
+  &&  [| ((Zlength (l2)) = cap2) |] 
+  &&  [| (cap2 >= n_pre) |] 
+  &&  [| (cap1 <= 100000000) |] 
+  &&  [| (cap2 <= 100000000) |] 
+  &&  [| (n_pre > 0) |] 
+  &&  [| (n_pre <= cap1) |]
+  &&  (store_uint_array_rec rp_pre i cap2 (replace_Znth ((i - i )) ((unsigned_last_nbits (((Znth i l_2 0) + b_pre )) (32))) (l'')) )
+  **  (store_uint_array ap_pre n_pre l_2 )
+  **  ((( &( "r" ) )) # UInt  |-> (unsigned_last_nbits (((Znth i l_2 0) + b_pre )) (32)))
+  **  ((( &( "i" ) )) # Int  |-> i)
+  **  (store_undef_uint_array_rec ap_pre n_pre cap1 )
+  **  (store_uint_array rp_pre i l' )
+  **  ((( &( "b" ) )) # UInt  |-> 1)
+  **  ((( &( "n" ) )) # Int  |-> n_pre)
+  **  ((( &( "ap" ) )) # Ptr  |-> ap_pre)
+  **  ((( &( "rp" ) )) # Ptr  |-> rp_pre)
+|--
+  [| ((i + 1 ) <= INT_MAX) |] 
+  &&  [| ((INT_MIN) <= (i + 1 )) |]
+.
+
+Definition mpn_add_1_entail_wit_1 := 
+forall (b_pre: Z) (n_pre: Z) (ap_pre: Z) (rp_pre: Z) (cap2: Z) (cap1: Z) (l2: (@list Z)) (val: Z) (l_2: (@list Z)) ,
+  [| ((Zlength (l2)) = cap2) |] 
+  &&  [| (n_pre <= cap1) |] 
+  &&  [| ((Zlength (l_2)) = n_pre) |] 
+  &&  [| (cap1 <= 100000000) |] 
+  &&  [| (list_store_Z_compact l_2 val ) |] 
+  &&  [| ((Zlength (l2)) = cap2) |] 
+  &&  [| (cap2 >= n_pre) |] 
+  &&  [| (cap1 <= 100000000) |] 
+  &&  [| (cap2 <= 100000000) |] 
+  &&  [| (n_pre > 0) |] 
+  &&  [| (n_pre <= cap1) |]
+  &&  (store_uint_array_rec rp_pre 0 cap2 l2 )
+  **  (store_uint_array rp_pre 0 nil )
+  **  (store_uint_array ap_pre n_pre l_2 )
+  **  (store_undef_uint_array_rec ap_pre n_pre cap1 )
+|--
+  EX (l'': (@list Z))  (l': (@list Z))  (val2: Z)  (val1: Z)  (l: (@list Z)) ,
+  [| (0 <= 0) |] 
+  &&  [| (0 <= n_pre) |] 
+  &&  [| (list_store_Z_compact l val ) |] 
+  &&  [| (n_pre <= cap1) |] 
+  &&  [| (list_store_Z (sublist (0) (0) (l)) val1 ) |] 
+  &&  [| (list_store_Z l' val2 ) |] 
+  &&  [| ((val2 + (b_pre * (Z.lxor UINT_MOD 0) ) ) = (val1 + b_pre )) |] 
+  &&  [| ((Zlength (l2)) = cap2) |] 
+  &&  [| (n_pre <= cap1) |] 
+  &&  [| ((Zlength (l_2)) = n_pre) |] 
+  &&  [| (cap1 <= 100000000) |] 
+  &&  [| (list_store_Z_compact l_2 val ) |] 
+  &&  [| ((Zlength (l2)) = cap2) |] 
+  &&  [| (cap2 >= n_pre) |] 
+  &&  [| (cap1 <= 100000000) |] 
+  &&  [| (cap2 <= 100000000) |] 
+  &&  [| (n_pre > 0) |] 
+  &&  [| (n_pre <= cap1) |]
+  &&  (store_uint_array ap_pre n_pre l )
+  **  (store_undef_uint_array_rec ap_pre n_pre cap1 )
+  **  (store_uint_array rp_pre 0 l' )
+  **  (store_uint_array_rec rp_pre 0 cap2 l'' )
+.
+
+Definition mpn_add_1_entail_wit_2_1 := 
+forall (b_pre: Z) (n_pre: Z) (ap_pre: Z) (rp_pre: Z) (cap2: Z) (cap1: Z) (l2: (@list Z)) (val: Z) (l_2: (@list Z)) (l''_2: (@list Z)) (l'_2: (@list Z)) (val2_2: Z) (val1_2: Z) (l_3: (@list Z)) (i: Z) ,
+  [| ((unsigned_last_nbits (((Znth i l_3 0) + b_pre )) (32)) < b_pre) |] 
+  &&  [| (i < n_pre) |] 
+  &&  [| (0 <= i) |] 
+  &&  [| (i <= n_pre) |] 
+  &&  [| (list_store_Z_compact l_3 val ) |] 
+  &&  [| (n_pre <= cap1) |] 
+  &&  [| (list_store_Z (sublist (0) (i) (l_3)) val1_2 ) |] 
+  &&  [| (list_store_Z l'_2 val2_2 ) |] 
+  &&  [| ((val2_2 + (b_pre * (Z.lxor UINT_MOD i) ) ) = (val1_2 + b_pre )) |] 
+  &&  [| ((Zlength (l2)) = cap2) |] 
+  &&  [| (n_pre <= cap1) |] 
+  &&  [| ((Zlength (l_2)) = n_pre) |] 
+  &&  [| (cap1 <= 100000000) |] 
+  &&  [| (list_store_Z_compact l_2 val ) |] 
+  &&  [| ((Zlength (l2)) = cap2) |] 
+  &&  [| (cap2 >= n_pre) |] 
+  &&  [| (cap1 <= 100000000) |] 
+  &&  [| (cap2 <= 100000000) |] 
+  &&  [| (n_pre > 0) |] 
+  &&  [| (n_pre <= cap1) |]
+  &&  (store_uint_array_rec rp_pre i cap2 (replace_Znth ((i - i )) ((unsigned_last_nbits (((Znth i l_3 0) + b_pre )) (32))) (l''_2)) )
+  **  (store_uint_array ap_pre n_pre l_3 )
+  **  (store_undef_uint_array_rec ap_pre n_pre cap1 )
+  **  (store_uint_array rp_pre i l'_2 )
+  **  ((( &( "b" ) )) # UInt  |-> 1)
+|--
+  EX (l'': (@list Z))  (l': (@list Z))  (val2: Z)  (val1: Z)  (l: (@list Z)) ,
+  [| (0 <= (i + 1 )) |] 
+  &&  [| ((i + 1 ) <= n_pre) |] 
+  &&  [| (list_store_Z_compact l val ) |] 
+  &&  [| (n_pre <= cap1) |] 
+  &&  [| (list_store_Z (sublist (0) ((i + 1 )) (l)) val1 ) |] 
+  &&  [| (list_store_Z l' val2 ) |] 
+  &&  [| ((val2 + (b_pre * (Z.lxor UINT_MOD (i + 1 )) ) ) = (val1 + b_pre )) |] 
+  &&  [| ((Zlength (l2)) = cap2) |] 
+  &&  [| (n_pre <= cap1) |] 
+  &&  [| ((Zlength (l_2)) = n_pre) |] 
+  &&  [| (cap1 <= 100000000) |] 
+  &&  [| (list_store_Z_compact l_2 val ) |] 
+  &&  [| ((Zlength (l2)) = cap2) |] 
+  &&  [| (cap2 >= n_pre) |] 
+  &&  [| (cap1 <= 100000000) |] 
+  &&  [| (cap2 <= 100000000) |] 
+  &&  [| (n_pre > 0) |] 
+  &&  [| (n_pre <= cap1) |]
+  &&  (store_uint_array ap_pre n_pre l )
+  **  (store_undef_uint_array_rec ap_pre n_pre cap1 )
+  **  (store_uint_array rp_pre (i + 1 ) l' )
+  **  (store_uint_array_rec rp_pre (i + 1 ) cap2 l'' )
+  **  ((( &( "b" ) )) # UInt  |-> b_pre)
+.
+
+Definition mpn_add_1_entail_wit_2_2 := 
+forall (b_pre: Z) (n_pre: Z) (ap_pre: Z) (rp_pre: Z) (cap2: Z) (cap1: Z) (l2: (@list Z)) (val: Z) (l_2: (@list Z)) (l''_2: (@list Z)) (l'_2: (@list Z)) (val2_2: Z) (val1_2: Z) (l_3: (@list Z)) (i: Z) ,
+  [| ((unsigned_last_nbits (((Znth i l_3 0) + b_pre )) (32)) >= b_pre) |] 
+  &&  [| (i < n_pre) |] 
+  &&  [| (0 <= i) |] 
+  &&  [| (i <= n_pre) |] 
+  &&  [| (list_store_Z_compact l_3 val ) |] 
+  &&  [| (n_pre <= cap1) |] 
+  &&  [| (list_store_Z (sublist (0) (i) (l_3)) val1_2 ) |] 
+  &&  [| (list_store_Z l'_2 val2_2 ) |] 
+  &&  [| ((val2_2 + (b_pre * (Z.lxor UINT_MOD i) ) ) = (val1_2 + b_pre )) |] 
+  &&  [| ((Zlength (l2)) = cap2) |] 
+  &&  [| (n_pre <= cap1) |] 
+  &&  [| ((Zlength (l_2)) = n_pre) |] 
+  &&  [| (cap1 <= 100000000) |] 
+  &&  [| (list_store_Z_compact l_2 val ) |] 
+  &&  [| ((Zlength (l2)) = cap2) |] 
+  &&  [| (cap2 >= n_pre) |] 
+  &&  [| (cap1 <= 100000000) |] 
+  &&  [| (cap2 <= 100000000) |] 
+  &&  [| (n_pre > 0) |] 
+  &&  [| (n_pre <= cap1) |]
+  &&  (store_uint_array_rec rp_pre i cap2 (replace_Znth ((i - i )) ((unsigned_last_nbits (((Znth i l_3 0) + b_pre )) (32))) (l''_2)) )
+  **  (store_uint_array ap_pre n_pre l_3 )
+  **  (store_undef_uint_array_rec ap_pre n_pre cap1 )
+  **  (store_uint_array rp_pre i l'_2 )
+  **  ((( &( "b" ) )) # UInt  |-> 0)
+|--
+  EX (l'': (@list Z))  (l': (@list Z))  (val2: Z)  (val1: Z)  (l: (@list Z)) ,
+  [| (0 <= (i + 1 )) |] 
+  &&  [| ((i + 1 ) <= n_pre) |] 
+  &&  [| (list_store_Z_compact l val ) |] 
+  &&  [| (n_pre <= cap1) |] 
+  &&  [| (list_store_Z (sublist (0) ((i + 1 )) (l)) val1 ) |] 
+  &&  [| (list_store_Z l' val2 ) |] 
+  &&  [| ((val2 + (b_pre * (Z.lxor UINT_MOD (i + 1 )) ) ) = (val1 + b_pre )) |] 
+  &&  [| ((Zlength (l2)) = cap2) |] 
+  &&  [| (n_pre <= cap1) |] 
+  &&  [| ((Zlength (l_2)) = n_pre) |] 
+  &&  [| (cap1 <= 100000000) |] 
+  &&  [| (list_store_Z_compact l_2 val ) |] 
+  &&  [| ((Zlength (l2)) = cap2) |] 
+  &&  [| (cap2 >= n_pre) |] 
+  &&  [| (cap1 <= 100000000) |] 
+  &&  [| (cap2 <= 100000000) |] 
+  &&  [| (n_pre > 0) |] 
+  &&  [| (n_pre <= cap1) |]
+  &&  (store_uint_array ap_pre n_pre l )
+  **  (store_undef_uint_array_rec ap_pre n_pre cap1 )
+  **  (store_uint_array rp_pre (i + 1 ) l' )
+  **  (store_uint_array_rec rp_pre (i + 1 ) cap2 l'' )
+  **  ((( &( "b" ) )) # UInt  |-> b_pre)
+.
+
+Definition mpn_add_1_return_wit_1 := 
+forall (b_pre: Z) (n_pre: Z) (ap_pre: Z) (rp_pre: Z) (cap2: Z) (cap1: Z) (l2: (@list Z)) (val: Z) (l_2: (@list Z)) (l'': (@list Z)) (l': (@list Z)) (val2: Z) (val1: Z) (l: (@list Z)) (i: Z) ,
+  [| (i >= n_pre) |] 
+  &&  [| (0 <= i) |] 
+  &&  [| (i <= n_pre) |] 
+  &&  [| (list_store_Z_compact l val ) |] 
+  &&  [| (n_pre <= cap1) |] 
+  &&  [| (list_store_Z (sublist (0) (i) (l)) val1 ) |] 
+  &&  [| (list_store_Z l' val2 ) |] 
+  &&  [| ((val2 + (b_pre * (Z.lxor UINT_MOD i) ) ) = (val1 + b_pre )) |] 
+  &&  [| ((Zlength (l2)) = cap2) |] 
+  &&  [| (n_pre <= cap1) |] 
+  &&  [| ((Zlength (l_2)) = n_pre) |] 
+  &&  [| (cap1 <= 100000000) |] 
+  &&  [| (list_store_Z_compact l_2 val ) |] 
+  &&  [| ((Zlength (l2)) = cap2) |] 
+  &&  [| (cap2 >= n_pre) |] 
+  &&  [| (cap1 <= 100000000) |] 
+  &&  [| (cap2 <= 100000000) |] 
+  &&  [| (n_pre > 0) |] 
+  &&  [| (n_pre <= cap1) |]
+  &&  (store_uint_array ap_pre n_pre l )
+  **  (store_undef_uint_array_rec ap_pre n_pre cap1 )
+  **  (store_uint_array rp_pre i l' )
+  **  (store_uint_array_rec rp_pre i cap2 l'' )
+|--
+  EX (val': Z) ,
+  [| ((val' + (b_pre * (Z.lxor UINT_MOD n_pre) ) ) = (val + b_pre )) |]
+  &&  (mpd_store_Z_compact ap_pre val n_pre cap1 )
+  **  (mpd_store_Z_compact rp_pre val' n_pre cap2 )
+.
+
+Definition mpn_add_1_partial_solve_wit_1 := 
+forall (n_pre: Z) (ap_pre: Z) (rp_pre: Z) (cap2: Z) (cap1: Z) (l2: (@list Z)) (val: Z) ,
+  [| ((Zlength (l2)) = cap2) |] 
+  &&  [| (cap2 >= n_pre) |] 
+  &&  [| (cap1 <= 100000000) |] 
+  &&  [| (cap2 <= 100000000) |] 
+  &&  [| (n_pre > 0) |] 
+  &&  [| (n_pre <= cap1) |]
+  &&  (mpd_store_Z_compact ap_pre val n_pre cap1 )
+  **  (store_uint_array rp_pre cap2 l2 )
+|--
+  [| ((Zlength (l2)) = cap2) |] 
+  &&  [| (cap2 >= n_pre) |] 
+  &&  [| (cap1 <= 100000000) |] 
+  &&  [| (cap2 <= 100000000) |] 
+  &&  [| (n_pre > 0) |] 
+  &&  [| (n_pre <= cap1) |]
+  &&  (mpd_store_Z_compact ap_pre val n_pre cap1 )
+  **  (store_uint_array rp_pre cap2 l2 )
+.
+
+Definition mpn_add_1_partial_solve_wit_2_pure := 
+forall (b_pre: Z) (n_pre: Z) (ap_pre: Z) (rp_pre: Z) (cap2: Z) (cap1: Z) (l2: (@list Z)) (val: Z) (l: (@list Z)) ,
+  [| (n_pre <= cap1) |] 
+  &&  [| ((Zlength (l)) = n_pre) |] 
+  &&  [| (cap1 <= 100000000) |] 
+  &&  [| (list_store_Z_compact l val ) |] 
+  &&  [| ((Zlength (l2)) = cap2) |] 
+  &&  [| (cap2 >= n_pre) |] 
+  &&  [| (cap1 <= 100000000) |] 
+  &&  [| (cap2 <= 100000000) |] 
+  &&  [| (n_pre > 0) |] 
+  &&  [| (n_pre <= cap1) |]
+  &&  ((( &( "i" ) )) # Int  |-> 0)
+  **  (store_uint_array ap_pre n_pre l )
+  **  (store_undef_uint_array_rec ap_pre n_pre cap1 )
+  **  ((( &( "b" ) )) # UInt  |-> b_pre)
+  **  ((( &( "n" ) )) # Int  |-> n_pre)
+  **  ((( &( "ap" ) )) # Ptr  |-> ap_pre)
+  **  ((( &( "rp" ) )) # Ptr  |-> rp_pre)
+  **  (store_uint_array rp_pre cap2 l2 )
+|--
+  [| ((Zlength (l2)) = cap2) |]
+.
+
+Definition mpn_add_1_partial_solve_wit_2_aux := 
+forall (n_pre: Z) (ap_pre: Z) (rp_pre: Z) (cap2: Z) (cap1: Z) (l2: (@list Z)) (val: Z) (l: (@list Z)) ,
+  [| (n_pre <= cap1) |] 
+  &&  [| ((Zlength (l)) = n_pre) |] 
+  &&  [| (cap1 <= 100000000) |] 
+  &&  [| (list_store_Z_compact l val ) |] 
+  &&  [| ((Zlength (l2)) = cap2) |] 
+  &&  [| (cap2 >= n_pre) |] 
+  &&  [| (cap1 <= 100000000) |] 
+  &&  [| (cap2 <= 100000000) |] 
+  &&  [| (n_pre > 0) |] 
+  &&  [| (n_pre <= cap1) |]
+  &&  (store_uint_array ap_pre n_pre l )
+  **  (store_undef_uint_array_rec ap_pre n_pre cap1 )
+  **  (store_uint_array rp_pre cap2 l2 )
+|--
+  [| ((Zlength (l2)) = cap2) |] 
+  &&  [| (n_pre <= cap1) |] 
+  &&  [| ((Zlength (l)) = n_pre) |] 
+  &&  [| (cap1 <= 100000000) |] 
+  &&  [| (list_store_Z_compact l val ) |] 
+  &&  [| ((Zlength (l2)) = cap2) |] 
+  &&  [| (cap2 >= n_pre) |] 
+  &&  [| (cap1 <= 100000000) |] 
+  &&  [| (cap2 <= 100000000) |] 
+  &&  [| (n_pre > 0) |] 
+  &&  [| (n_pre <= cap1) |]
+  &&  (store_uint_array rp_pre cap2 l2 )
+  **  (store_uint_array ap_pre n_pre l )
+  **  (store_undef_uint_array_rec ap_pre n_pre cap1 )
+.
+
+Definition mpn_add_1_partial_solve_wit_2 := mpn_add_1_partial_solve_wit_2_pure -> mpn_add_1_partial_solve_wit_2_aux.
+
+Definition mpn_add_1_partial_solve_wit_3 := 
+forall (b_pre: Z) (n_pre: Z) (ap_pre: Z) (rp_pre: Z) (cap2: Z) (cap1: Z) (l2: (@list Z)) (val: Z) (l: (@list Z)) (l'': (@list Z)) (l': (@list Z)) (val2: Z) (val1: Z) (l_2: (@list Z)) (i: Z) ,
+  [| (i < n_pre) |] 
+  &&  [| (0 <= i) |] 
+  &&  [| (i <= n_pre) |] 
+  &&  [| (list_store_Z_compact l_2 val ) |] 
+  &&  [| (n_pre <= cap1) |] 
+  &&  [| (list_store_Z (sublist (0) (i) (l_2)) val1 ) |] 
+  &&  [| (list_store_Z l' val2 ) |] 
+  &&  [| ((val2 + (b_pre * (Z.lxor UINT_MOD i) ) ) = (val1 + b_pre )) |] 
+  &&  [| ((Zlength (l2)) = cap2) |] 
+  &&  [| (n_pre <= cap1) |] 
+  &&  [| ((Zlength (l)) = n_pre) |] 
+  &&  [| (cap1 <= 100000000) |] 
+  &&  [| (list_store_Z_compact l val ) |] 
+  &&  [| ((Zlength (l2)) = cap2) |] 
+  &&  [| (cap2 >= n_pre) |] 
+  &&  [| (cap1 <= 100000000) |] 
+  &&  [| (cap2 <= 100000000) |] 
+  &&  [| (n_pre > 0) |] 
+  &&  [| (n_pre <= cap1) |]
+  &&  (store_uint_array ap_pre n_pre l_2 )
+  **  (store_undef_uint_array_rec ap_pre n_pre cap1 )
+  **  (store_uint_array rp_pre i l' )
+  **  (store_uint_array_rec rp_pre i cap2 l'' )
+|--
+  [| (i < n_pre) |] 
+  &&  [| (0 <= i) |] 
+  &&  [| (i <= n_pre) |] 
+  &&  [| (list_store_Z_compact l_2 val ) |] 
+  &&  [| (n_pre <= cap1) |] 
+  &&  [| (list_store_Z (sublist (0) (i) (l_2)) val1 ) |] 
+  &&  [| (list_store_Z l' val2 ) |] 
+  &&  [| ((val2 + (b_pre * (Z.lxor UINT_MOD i) ) ) = (val1 + b_pre )) |] 
+  &&  [| ((Zlength (l2)) = cap2) |] 
+  &&  [| (n_pre <= cap1) |] 
+  &&  [| ((Zlength (l)) = n_pre) |] 
+  &&  [| (cap1 <= 100000000) |] 
+  &&  [| (list_store_Z_compact l val ) |] 
+  &&  [| ((Zlength (l2)) = cap2) |] 
+  &&  [| (cap2 >= n_pre) |] 
+  &&  [| (cap1 <= 100000000) |] 
+  &&  [| (cap2 <= 100000000) |] 
+  &&  [| (n_pre > 0) |] 
+  &&  [| (n_pre <= cap1) |]
+  &&  (((ap_pre + (i * sizeof(UINT) ) )) # UInt  |-> (Znth i l_2 0))
+  **  (store_uint_array_missing_i_rec ap_pre i 0 n_pre l_2 )
+  **  (store_undef_uint_array_rec ap_pre n_pre cap1 )
+  **  (store_uint_array rp_pre i l' )
+  **  (store_uint_array_rec rp_pre i cap2 l'' )
+.
+
+Definition mpn_add_1_partial_solve_wit_4 := 
+forall (b_pre: Z) (n_pre: Z) (ap_pre: Z) (rp_pre: Z) (cap2: Z) (cap1: Z) (l2: (@list Z)) (val: Z) (l: (@list Z)) (l'': (@list Z)) (l': (@list Z)) (val2: Z) (val1: Z) (l_2: (@list Z)) (i: Z) ,
+  [| ((unsigned_last_nbits (((Znth i l_2 0) + b_pre )) (32)) < b_pre) |] 
+  &&  [| (i < n_pre) |] 
+  &&  [| (0 <= i) |] 
+  &&  [| (i <= n_pre) |] 
+  &&  [| (list_store_Z_compact l_2 val ) |] 
+  &&  [| (n_pre <= cap1) |] 
+  &&  [| (list_store_Z (sublist (0) (i) (l_2)) val1 ) |] 
+  &&  [| (list_store_Z l' val2 ) |] 
+  &&  [| ((val2 + (b_pre * (Z.lxor UINT_MOD i) ) ) = (val1 + b_pre )) |] 
+  &&  [| ((Zlength (l2)) = cap2) |] 
+  &&  [| (n_pre <= cap1) |] 
+  &&  [| ((Zlength (l)) = n_pre) |] 
+  &&  [| (cap1 <= 100000000) |] 
+  &&  [| (list_store_Z_compact l val ) |] 
+  &&  [| ((Zlength (l2)) = cap2) |] 
+  &&  [| (cap2 >= n_pre) |] 
+  &&  [| (cap1 <= 100000000) |] 
+  &&  [| (cap2 <= 100000000) |] 
+  &&  [| (n_pre > 0) |] 
+  &&  [| (n_pre <= cap1) |]
+  &&  (store_uint_array ap_pre n_pre l_2 )
+  **  (store_undef_uint_array_rec ap_pre n_pre cap1 )
+  **  (store_uint_array rp_pre i l' )
+  **  (store_uint_array_rec rp_pre i cap2 l'' )
+|--
+  [| ((unsigned_last_nbits (((Znth i l_2 0) + b_pre )) (32)) < b_pre) |] 
+  &&  [| (i < n_pre) |] 
+  &&  [| (0 <= i) |] 
+  &&  [| (i <= n_pre) |] 
+  &&  [| (list_store_Z_compact l_2 val ) |] 
+  &&  [| (n_pre <= cap1) |] 
+  &&  [| (list_store_Z (sublist (0) (i) (l_2)) val1 ) |] 
+  &&  [| (list_store_Z l' val2 ) |] 
+  &&  [| ((val2 + (b_pre * (Z.lxor UINT_MOD i) ) ) = (val1 + b_pre )) |] 
+  &&  [| ((Zlength (l2)) = cap2) |] 
+  &&  [| (n_pre <= cap1) |] 
+  &&  [| ((Zlength (l)) = n_pre) |] 
+  &&  [| (cap1 <= 100000000) |] 
+  &&  [| (list_store_Z_compact l val ) |] 
+  &&  [| ((Zlength (l2)) = cap2) |] 
+  &&  [| (cap2 >= n_pre) |] 
+  &&  [| (cap1 <= 100000000) |] 
+  &&  [| (cap2 <= 100000000) |] 
+  &&  [| (n_pre > 0) |] 
+  &&  [| (n_pre <= cap1) |]
+  &&  (((rp_pre + (i * sizeof(UINT) ) )) # UInt  |->_)
+  **  (store_uint_array_missing_i_rec rp_pre i i cap2 l'' )
+  **  (store_uint_array ap_pre n_pre l_2 )
+  **  (store_undef_uint_array_rec ap_pre n_pre cap1 )
+  **  (store_uint_array rp_pre i l' )
+.
+
+Definition mpn_add_1_partial_solve_wit_5 := 
+forall (b_pre: Z) (n_pre: Z) (ap_pre: Z) (rp_pre: Z) (cap2: Z) (cap1: Z) (l2: (@list Z)) (val: Z) (l: (@list Z)) (l'': (@list Z)) (l': (@list Z)) (val2: Z) (val1: Z) (l_2: (@list Z)) (i: Z) ,
+  [| ((unsigned_last_nbits (((Znth i l_2 0) + b_pre )) (32)) >= b_pre) |] 
+  &&  [| (i < n_pre) |] 
+  &&  [| (0 <= i) |] 
+  &&  [| (i <= n_pre) |] 
+  &&  [| (list_store_Z_compact l_2 val ) |] 
+  &&  [| (n_pre <= cap1) |] 
+  &&  [| (list_store_Z (sublist (0) (i) (l_2)) val1 ) |] 
+  &&  [| (list_store_Z l' val2 ) |] 
+  &&  [| ((val2 + (b_pre * (Z.lxor UINT_MOD i) ) ) = (val1 + b_pre )) |] 
+  &&  [| ((Zlength (l2)) = cap2) |] 
+  &&  [| (n_pre <= cap1) |] 
+  &&  [| ((Zlength (l)) = n_pre) |] 
+  &&  [| (cap1 <= 100000000) |] 
+  &&  [| (list_store_Z_compact l val ) |] 
+  &&  [| ((Zlength (l2)) = cap2) |] 
+  &&  [| (cap2 >= n_pre) |] 
+  &&  [| (cap1 <= 100000000) |] 
+  &&  [| (cap2 <= 100000000) |] 
+  &&  [| (n_pre > 0) |] 
+  &&  [| (n_pre <= cap1) |]
+  &&  (store_uint_array ap_pre n_pre l_2 )
+  **  (store_undef_uint_array_rec ap_pre n_pre cap1 )
+  **  (store_uint_array rp_pre i l' )
+  **  (store_uint_array_rec rp_pre i cap2 l'' )
+|--
+  [| ((unsigned_last_nbits (((Znth i l_2 0) + b_pre )) (32)) >= b_pre) |] 
+  &&  [| (i < n_pre) |] 
+  &&  [| (0 <= i) |] 
+  &&  [| (i <= n_pre) |] 
+  &&  [| (list_store_Z_compact l_2 val ) |] 
+  &&  [| (n_pre <= cap1) |] 
+  &&  [| (list_store_Z (sublist (0) (i) (l_2)) val1 ) |] 
+  &&  [| (list_store_Z l' val2 ) |] 
+  &&  [| ((val2 + (b_pre * (Z.lxor UINT_MOD i) ) ) = (val1 + b_pre )) |] 
+  &&  [| ((Zlength (l2)) = cap2) |] 
+  &&  [| (n_pre <= cap1) |] 
+  &&  [| ((Zlength (l)) = n_pre) |] 
+  &&  [| (cap1 <= 100000000) |] 
+  &&  [| (list_store_Z_compact l val ) |] 
+  &&  [| ((Zlength (l2)) = cap2) |] 
+  &&  [| (cap2 >= n_pre) |] 
+  &&  [| (cap1 <= 100000000) |] 
+  &&  [| (cap2 <= 100000000) |] 
+  &&  [| (n_pre > 0) |] 
+  &&  [| (n_pre <= cap1) |]
+  &&  (((rp_pre + (i * sizeof(UINT) ) )) # UInt  |->_)
+  **  (store_uint_array_missing_i_rec rp_pre i i cap2 l'' )
+  **  (store_uint_array ap_pre n_pre l_2 )
+  **  (store_undef_uint_array_rec ap_pre n_pre cap1 )
+  **  (store_uint_array rp_pre i l' )
+.
+
+Definition mpn_add_1_which_implies_wit_1 := 
+forall (n_pre: Z) (ap_pre: Z) (cap1: Z) (val: Z) ,
+  (mpd_store_Z_compact ap_pre val n_pre cap1 )
+|--
+  EX (l: (@list Z)) ,
+  [| (n_pre <= cap1) |] 
+  &&  [| ((Zlength (l)) = n_pre) |] 
+  &&  [| (cap1 <= 100000000) |] 
+  &&  [| (list_store_Z_compact l val ) |]
+  &&  (store_uint_array ap_pre n_pre l )
+  **  (store_undef_uint_array_rec ap_pre n_pre cap1 )
+.
+
+Definition mpn_add_1_which_implies_wit_2 := 
+forall (rp_pre: Z) (cap2: Z) (l2: (@list Z)) ,
+  [| ((Zlength (l2)) = cap2) |]
+  &&  (store_uint_array rp_pre cap2 l2 )
+|--
+  [| ((Zlength (l2)) = cap2) |]
+  &&  (store_uint_array_rec rp_pre 0 cap2 l2 )
+  **  (store_uint_array rp_pre 0 nil )
+.
+
 Module Type VC_Correct.
 
 Axiom proof_of_gmp_abs_safety_wit_1 : gmp_abs_safety_wit_1.
@@ -1823,5 +2369,20 @@ Axiom proof_of_mpn_normalized_size_return_wit_1_2 : mpn_normalized_size_return_w
 Axiom proof_of_mpn_normalized_size_partial_solve_wit_1 : mpn_normalized_size_partial_solve_wit_1.
 Axiom proof_of_mpn_normalized_size_partial_solve_wit_2 : mpn_normalized_size_partial_solve_wit_2.
 Axiom proof_of_mpn_normalized_size_which_implies_wit_1 : mpn_normalized_size_which_implies_wit_1.
+Axiom proof_of_mpn_add_1_safety_wit_1 : mpn_add_1_safety_wit_1.
+Axiom proof_of_mpn_add_1_safety_wit_2 : mpn_add_1_safety_wit_2.
+Axiom proof_of_mpn_add_1_safety_wit_3 : mpn_add_1_safety_wit_3.
+Axiom proof_of_mpn_add_1_entail_wit_1 : mpn_add_1_entail_wit_1.
+Axiom proof_of_mpn_add_1_entail_wit_2_1 : mpn_add_1_entail_wit_2_1.
+Axiom proof_of_mpn_add_1_entail_wit_2_2 : mpn_add_1_entail_wit_2_2.
+Axiom proof_of_mpn_add_1_return_wit_1 : mpn_add_1_return_wit_1.
+Axiom proof_of_mpn_add_1_partial_solve_wit_1 : mpn_add_1_partial_solve_wit_1.
+Axiom proof_of_mpn_add_1_partial_solve_wit_2_pure : mpn_add_1_partial_solve_wit_2_pure.
+Axiom proof_of_mpn_add_1_partial_solve_wit_2 : mpn_add_1_partial_solve_wit_2.
+Axiom proof_of_mpn_add_1_partial_solve_wit_3 : mpn_add_1_partial_solve_wit_3.
+Axiom proof_of_mpn_add_1_partial_solve_wit_4 : mpn_add_1_partial_solve_wit_4.
+Axiom proof_of_mpn_add_1_partial_solve_wit_5 : mpn_add_1_partial_solve_wit_5.
+Axiom proof_of_mpn_add_1_which_implies_wit_1 : mpn_add_1_which_implies_wit_1.
+Axiom proof_of_mpn_add_1_which_implies_wit_2 : mpn_add_1_which_implies_wit_2.
 
 End VC_Correct.
