projects/lib/gmp_proof_auto.v
@@ -15,6 +15,8 @@ Local Open Scope Z_scope.
 Local Open Scope sets.
 Local Open Scope string.
 Local Open Scope list.
+Require Import Coq.ZArith.ZArith.
+Local Open Scope Z_scope.
 Import naive_C_Rules.
 Local Open Scope sac.
 
@@ -139,5 +141,32 @@ Lemma proof_of_mpn_normalized_size_partial_solve_wit_1 : mpn_normalized_size_par
 Proof. Admitted. 
 
 Lemma proof_of_mpn_normalized_size_partial_solve_wit_2 : mpn_normalized_size_partial_solve_wit_2.
+Proof. Admitted. 
+
+Lemma proof_of_mpn_add_1_safety_wit_1 : mpn_add_1_safety_wit_1.
+Proof. Admitted. 
+
+Lemma proof_of_mpn_add_1_safety_wit_2 : mpn_add_1_safety_wit_2.
+Proof. Admitted. 
+
+Lemma proof_of_mpn_add_1_safety_wit_3 : mpn_add_1_safety_wit_3.
+Proof. Admitted. 
+
+Lemma proof_of_mpn_add_1_partial_solve_wit_1 : mpn_add_1_partial_solve_wit_1.
+Proof. Admitted. 
+
+Lemma proof_of_mpn_add_1_partial_solve_wit_2_pure : mpn_add_1_partial_solve_wit_2_pure.
+Proof. Admitted. 
+
+Lemma proof_of_mpn_add_1_partial_solve_wit_2 : mpn_add_1_partial_solve_wit_2.
+Proof. Admitted. 
+
+Lemma proof_of_mpn_add_1_partial_solve_wit_3 : mpn_add_1_partial_solve_wit_3.
+Proof. Admitted. 
+
+Lemma proof_of_mpn_add_1_partial_solve_wit_4 : mpn_add_1_partial_solve_wit_4.
+Proof. Admitted. 
+
+Lemma proof_of_mpn_add_1_partial_solve_wit_5 : mpn_add_1_partial_solve_wit_5.
 Proof. Admitted. 
 
